split off context extension as a separate relation
the inference system is now dependent only on the theory (not a specific
list of updates, just the signature and the axioms) and does not update
the context. it is proved sound for an unchanging theory. a separate
relation defines the updates to a context that will be syntactically
allowed. have not proved soundness for these updates yet.

hol-light/stateful/holSemanticsScript.sml
@@ -76,24 +76,28 @@ val _ = Parse.overload_on("is_term_valuation",``is_term_valuation0 ^mem``)
    A valuation is a pair of valuations. *)
 
 val _ = Parse.type_abbrev("interpretation",``:'U tyass # 'U tmass``)
+val _ = Parse.overload_on("tyaof",``FST:'U interpretation->'U tyass``)
+val _ = Parse.overload_on("tmaof",``SND:'U interpretation->'U tmass``)
 val _ = Parse.type_abbrev("valuation",``:'U tyval # 'U tmval``)
+val _ = Parse.overload_on("tyvof",``FST:'U valuation->'U tyval``)
+val _ = Parse.overload_on("tmvof",``SND:'U valuation->'U tmval``)
 
 val is_valuation_def = xDefine"is_valuation"`
-  is_valuation0 ^mem δ (τ,σ) ⇔
-    is_type_valuation τ ∧
-    is_term_valuation δ τ σ`
+  is_valuation0 ^mem δ v ⇔
+    is_type_valuation (tyvof v) ∧
+    is_term_valuation δ (tyvof v) (tmvof v)`
 val _ = Parse.overload_on("is_valuation",``is_valuation0 ^mem``)
 
 (* term assignment for instances of constants *)
 
 val instance_def = new_specification("instance_def",["instance"],
   prove(``∃f. ∀(Γ:sig) (i:'U interpretation) name ty ty0 tyin.
-              FLOOKUP (SND Γ) name = SOME ty0 ∧
+              FLOOKUP (tmsof Γ) name = SOME ty0 ∧
               ty = TYPE_SUBST tyin ty0
               ⇒
               f Γ i name ty =
-              λτ. (SND i) name (λx. if MEM x (tyvars ty0)
-                                    then typesem (FST i) τ (TYPE_SUBST tyin (Tyvar x))
+              λτ. tmaof i name (λx. if MEM x (tyvars ty0)
+                                    then typesem (tyaof i) τ (TYPE_SUBST tyin (Tyvar x))
                                     else ARB)``,
     simp[GSYM SKOLEM_THM] >> rw[] >>
     Cases_on`FLOOKUP (SND Γ) name`>>simp[] >>
@@ -108,20 +112,20 @@ val instance_def = new_specification("instance_def",["instance"],
 (* Semantics of terms. *)
 
 val termsem_def = xDefine "termsem"`
-  (termsem0 ^mem Γ (i:'U interpretation) (v:'U valuation) (Var x ty) = SND v (x,ty)) ∧
-  (termsem0 ^mem Γ i v (Const name ty) = instance Γ i name ty (FST v)) ∧
+  (termsem0 ^mem Γ (i:'U interpretation) (v:'U valuation) (Var x ty) = tmvof v (x,ty)) ∧
+  (termsem0 ^mem Γ i v (Const name ty) = instance Γ i name ty (tyvof v)) ∧
   (termsem0 ^mem Γ i v (Comb t1 t2) =
    termsem0 ^mem Γ i v t1 ' (termsem0 ^mem Γ i v t2)) ∧
   (termsem0 ^mem Γ i v (Abs x ty b) =
-   Abstract (typesem (FST i) (FST v) ty) (typesem (FST i) (FST v) (typeof b))
-     (λm. termsem0 ^mem Γ i (FST v, ((x,ty)=+m)(SND v)) b))`
+   Abstract (typesem (tyaof i) (tyvof v) ty) (typesem (tyaof i) (tyvof v) (typeof b))
+     (λm. termsem0 ^mem Γ i (tyvof v, ((x,ty)=+m)(tmvof v)) b))`
 val _ = Parse.overload_on("termsem",``termsem0 ^mem``)
 
 (* Satisfaction of sequents. *)
 
 val satisfies_def = xDefine"satisfies"`
-  satisfies0 ^mem (sig,i) (h,c) ⇔
-    ∀v. is_valuation (FST i) v ∧
+  satisfies0 ^mem i (sig,h,c) ⇔
+    ∀v. is_valuation (tyaof i) v ∧
       EVERY (λt. termsem sig i v t = True) h
       ⇒ termsem sig i v c = True`
 val _ = Parse.add_infix("satisfies",450,Parse.NONASSOC)
@@ -131,9 +135,9 @@ val _ = Parse.overload_on("satisfies",``satisfies0 ^mem``)
    types in the theory. *)
 
 val is_interpretation_def = xDefine "is_interpretation"`
-  is_interpretation0 ^mem (tyenv,tmenv) (δ,γ) ⇔
-    is_type_assignment tyenv δ ∧
-    is_term_assignment tmenv δ γ`
+  is_interpretation0 ^mem (sig:sig) int ⇔
+    is_type_assignment (tysof sig) (tyaof int) ∧
+    is_term_assignment (tmsof sig) (tyaof int) (tmaof int)`
 val _ = Parse.overload_on("is_interpretation",``is_interpretation0 ^mem``)
 
 (* The assignments are standard if they interpret fun, bool, and = according
@@ -146,9 +150,9 @@ val is_std_type_assignment_def = xDefine "is_std_type_assignment"`
 val _ = Parse.overload_on("is_std_type_assignment",``is_std_type_assignment0 ^mem``)
 
 val is_std_interpretation_def = xDefine "is_std_interpretation"`
-  is_std_interpretation0 ^mem ((δ,γ):'U interpretation) ⇔
-    is_std_type_assignment δ ∧
-    γ "=" = λτ.
+  is_std_interpretation0 ^mem (i:'U interpretation) ⇔
+    is_std_type_assignment (tyaof i) ∧
+    tmaof i "=" = λτ.
         (Abstract (τ"A") (Funspace (τ"A") boolset)
           (λx. Abstract (τ"A") boolset (λy. Boolean (x = y))))`
 val _ = Parse.overload_on("is_std_interpretation",``is_std_interpretation0 ^mem``)
@@ -156,22 +160,23 @@ val _ = Parse.overload_on("is_std_interpretation",``is_std_interpretation0 ^mem`
 (* A model of a theory is a standard interpretation that satisfies all the
    axioms. *)
 
-val is_model_def = xDefine"is_model"`
-  is_model0 ^mem (sig, axs) i ⇔
-    is_interpretation sig i ∧
+val models_def = xDefine"models"`
+  models0 ^mem i (thy:thy) ⇔
+    is_interpretation (sigof thy) i ∧
     is_std_interpretation i ∧
-    EVERY (λp. (sig,i) satisfies ([],p)) axs`
-val _ = Parse.overload_on("is_model",``is_model0 ^mem``)
+    ∀p. p ∈ (axsof thy) ⇒ i satisfies (sigof thy,[],p)`
+val _ = Parse.add_infix("models",450,Parse.NONASSOC)
+val _ = Parse.overload_on("models",``models0 ^mem``)
 
 (* Validity of sequents. *)
 
 val entails_def = xDefine"entails"`
-  entails0 ^mem (ctxt,h) c ⇔
-    context_ok ctxt ∧
-    EVERY (term_ok (sigof ctxt)) (c::h) ∧
-    EVERY (λt. t has_type Bool) (c::h) ∧
-    ∀i. is_model (sigof ctxt, axioms ctxt) i
-        ⇒ (sigof ctxt, i) satisfies (h,c)`
+  entails0 ^mem (thy,h) c ⇔
+    theory_ok thy ∧
+    EVERY (term_ok (sigof thy)) (c::h) ∧
+    EVERY (λp. p has_type Bool) (c::h) ∧
+    ∀i. i models thy
+        ⇒ i satisfies (sigof thy,h,c)`
 val _ = Parse.add_infix("|=",450,Parse.NONASSOC)
 val _ = Parse.overload_on("|=",``entails0 ^mem``)
 
@@ -183,7 +188,7 @@ val is_structure_def = xDefine"is_structure"`
     is_std_sig sig ∧
     is_std_interpretation int ∧
     is_interpretation sig int ∧
-    is_valuation (FST int) val`
+    is_valuation (tyaof int) val`
 val _ = Parse.overload_on("is_structure",``is_structure0 ^mem``)
 
 val _ = export_theory()
