hol-light/stateful/holSoundnessScript.sml
@@ -5,46 +5,40 @@ val _ = new_theory"holSoundness"
 
 val mem = ``mem:'U->'U-> bool``
 
-(* TODO: move *)
-val IS_SUFFIX_CONS = store_thm("IS_SUFFIX_CONS",
-  ``∀l1 l2 a. IS_SUFFIX l1 l2 ⇒ IS_SUFFIX (a::l1) l2``,
-  rw[rich_listTheory.IS_SUFFIX_APPEND] >>
-  qexists_tac`a::l` >>rw[])
-
 val binary_inference_rule = store_thm("binary_inference_rule",
   ``is_set_theory ^mem ⇒
-    ∀ctxt h1 h2 p1 p2 q.
-    q has_type Bool ∧ term_ok (sigof ctxt) q ∧
-    (∀i v. is_structure (sigof ctxt) i v ∧
-           termsem (sigof ctxt) i v p1 = True ∧
-           termsem (sigof ctxt) i v p2 = True ⇒
-           termsem (sigof ctxt) i v q = True) ∧
-    (ctxt,h1) |= p1 ∧ (ctxt,h2) |= p2
-    ⇒ (ctxt, TERM_UNION h1 h2) |= q``,
+    ∀thy h1 h2 p1 p2 q.
+    q has_type Bool ∧ term_ok (sigof thy) q ∧
+    (∀i v. is_structure (sigof thy) i v ∧
+           termsem (sigof thy) i v p1 = True ∧
+           termsem (sigof thy) i v p2 = True ⇒
+           termsem (sigof thy) i v q = True) ∧
+    (thy,h1) |= p1 ∧ (thy,h2) |= p2
+    ⇒ (thy, TERM_UNION h1 h2) |= q``,
   strip_tac >>
   rpt gen_tac >> strip_tac >>
   fs[entails_def,EVERY_TERM_UNION] >> rw[] >>
   rpt (first_x_assum(qspec_then`i`mp_tac)>>rw[]) >>
   fs[satisfies_def,EVERY_TERM_UNION] >> rw[] >>
   first_x_assum match_mp_tac >>
-  conj_tac >- ( rw[is_structure_def] >> fs[is_model_def,context_ok_sig] ) >>
+  conj_tac >- ( rw[is_structure_def] >> Cases_on`thy` >> fs[models_def,theory_ok_def] ) >>
   rw[] >> first_x_assum match_mp_tac >> rw[] >>
   fs[EVERY_MEM] >>
   metis_tac[TERM_UNION_NONEW,TERM_UNION_THM,termsem_aconv,welltyped_def])
 
 val ABS_correct = store_thm("ABS_correct",
   ``is_set_theory ^mem ⇒
-    ∀ctxt x ty h l r.
-    ¬EXISTS (VFREE_IN (Var x ty)) h ∧ type_ok (types ctxt) ty ∧
-    (ctxt,h) |= l === r
-    ⇒ (ctxt,h) |= Abs x ty l === Abs x ty r``,
+    ∀thy x ty h l r.
+    ¬EXISTS (VFREE_IN (Var x ty)) h ∧ type_ok (tysof thy) ty ∧
+    (thy,h) |= l === r
+    ⇒ (thy,h) |= Abs x ty l === Abs x ty r``,
   rw[] >> fs[entails_def] >>
-  imp_res_tac context_ok_sig >>
+  imp_res_tac theory_ok_sig >>
   conj_asm1_tac >- fs[term_ok_equation,term_ok_def] >>
   conj_asm1_tac >- fs[EQUATION_HAS_TYPE_BOOL] >> rw[] >>
   fs[satisfies_def] >> rw[] >>
-  `is_structure (sigof ctxt) i v` by (
-    fs[is_model_def,is_structure_def] ) >>
+  `is_structure (sigof thy) i v` by (
+    fs[models_def,is_structure_def] ) >>
   imp_res_tac termsem_equation >>
   rw[boolean_eq_true,termsem_def] >>
   match_mp_tac (UNDISCH abstract_eq) >>
@@ -61,35 +55,35 @@ val ABS_correct = store_thm("ABS_correct",
              ,pairTheory.FST,term_ok_equation]) >>
   first_x_assum(qspec_then`i`mp_tac) >> simp[] >>
   disch_then(qspec_then`vv`mp_tac) >> simp[] >>
-  `is_structure (sigof ctxt) i vv` by (
+  `is_structure (sigof thy) i vv` by (
     fs[is_structure_def] ) >>
   imp_res_tac (UNDISCH termsem_equation) >>
   simp[boolean_eq_true] >> disch_then match_mp_tac >>
   fs[EVERY_MEM] >> rw[] >>
-  qsuff_tac`termsem (sigof ctxt) i vv t = termsem (sigof ctxt) i v t`>-metis_tac[] >>
+  qsuff_tac`termsem (sigof thy) i vv t = termsem (sigof thy) i v t`>-metis_tac[] >>
   match_mp_tac termsem_frees >>
   simp[Abbr`vv`,combinTheory.APPLY_UPDATE_THM] >>
   rw[] >> metis_tac[])
 
 val ASSUME_correct = store_thm("ASSUME_correct",
-  ``∀ctxt p.
-      context_ok ctxt ∧ p has_type Bool ∧ term_ok (sigof ctxt) p
-      ⇒ (ctxt,[p]) |= p``,
+  ``∀thy p.
+      theory_ok thy ∧ p has_type Bool ∧ term_ok (sigof thy) p
+      ⇒ (thy,[p]) |= p``,
   rw[entails_def,satisfies_def])
 
 val BETA_correct = store_thm("BETA_correct",
   ``is_set_theory ^mem ⇒
-    ∀ctxt x ty t.
-      context_ok ctxt ∧ type_ok (types ctxt) ty ∧ term_ok (sigof ctxt) t ⇒
-      (ctxt,[]) |= Comb (Abs x ty t) (Var x ty) === t``,
+    ∀thy x ty t.
+      theory_ok thy ∧ type_ok (tysof thy) ty ∧ term_ok (sigof thy) t ⇒
+      (thy,[]) |= Comb (Abs x ty t) (Var x ty) === t``,
   rw[] >> simp[entails_def] >>
-  imp_res_tac context_ok_sig >>
+  imp_res_tac theory_ok_sig >>
   imp_res_tac term_ok_welltyped >>
   conj_asm1_tac >- ( simp[term_ok_equation,term_ok_def] ) >>
   conj_asm1_tac >- ( simp[EQUATION_HAS_TYPE_BOOL] ) >>
   rw[satisfies_def] >>
-  `is_structure (sigof ctxt) i v` by (
-    rw[is_structure_def] >> fs[is_model_def] ) >>
+  `is_structure (sigof thy) i v` by (
+    rw[is_structure_def] >> fs[models_def] ) >>
   imp_res_tac (UNDISCH termsem_equation) >>
   rw[boolean_eq_true,termsem_def] >>
   qmatch_abbrev_tac`(Abstract mty mtyb f ' e) = termsem Γ i v τ` >>
@@ -111,14 +105,14 @@ val BETA_correct = store_thm("BETA_correct",
 
 val DEDUCT_ANTISYM_correct = store_thm("DEDUCT_ANTISYM_correct",
   ``is_set_theory ^mem ⇒
-    ∀ctxt h1 p1 h2 p2.
-      (ctxt,h1) |= p1 ∧ (ctxt,h2) |= p2 ⇒
-      (ctxt,
+    ∀thy h1 p1 h2 p2.
+      (thy,h1) |= p1 ∧ (thy,h2) |= p2 ⇒
+      (thy,
        TERM_UNION (FILTER ($~ o ACONV p2) h1)
                   (FILTER ($~ o ACONV p1) h2))
       |= p1 === p2``,
   rw[] >> fs[entails_def] >>
-  imp_res_tac context_ok_sig >>
+  imp_res_tac theory_ok_sig >>
   conj_asm1_tac >- (
     simp[term_ok_equation] >>
     imp_res_tac WELLTYPED_LEMMA >> simp[] >>
@@ -130,8 +124,8 @@ val DEDUCT_ANTISYM_correct = store_thm("DEDUCT_ANTISYM_correct",
     match_mp_tac EVERY_TERM_UNION >>
     fs[EVERY_MEM,MEM_FILTER] ) >>
   rw[satisfies_def] >>
-  `is_structure (sigof ctxt) i v` by (
-    fs[is_model_def,is_structure_def] ) >>
+  `is_structure (sigof thy) i v` by (
+    fs[models_def,is_structure_def] ) >>
   imp_res_tac (UNDISCH termsem_equation) >>
   simp[boolean_eq_true] >>
   rpt(first_x_assum(qspec_then`i`mp_tac)>>rw[]) >>
@@ -147,8 +141,8 @@ val DEDUCT_ANTISYM_correct = store_thm("DEDUCT_ANTISYM_correct",
   `b ⇒ c` by (
     unabbrev_all_tac >> rw[] >>
     metis_tac[TERM_UNION_THM,termsem_aconv,welltyped_def] ) >>
-  `termsem (sigof ctxt) i v p1 <: boolset ∧
-   termsem (sigof ctxt) i v p2 <: boolset` by (
+  `termsem (sigof thy) i v p1 <: boolset ∧
+   termsem (sigof thy) i v p2 <: boolset` by (
     fs[is_structure_def] >>
     imp_res_tac is_std_interpretation_is_type >>
     imp_res_tac termsem_typesem >>
@@ -158,37 +152,36 @@ val DEDUCT_ANTISYM_correct = store_thm("DEDUCT_ANTISYM_correct",
 
 val EQ_MP_correct = store_thm("EQ_MP_correct",
   ``is_set_theory ^mem ⇒
-    ∀ctxt h1 h2 p q p'.
-      (ctxt,h1) |= p === q ∧ (ctxt,h2) |= p' ∧ ACONV p p' ⇒
-      (ctxt,TERM_UNION h1 h2) |= q``,
+    ∀thy h1 h2 p q p'.
+      (thy,h1) |= p === q ∧ (thy,h2) |= p' ∧ ACONV p p' ⇒
+      (thy,TERM_UNION h1 h2) |= q``,
   rw[] >>
   match_mp_tac (UNDISCH binary_inference_rule) >>
   map_every qexists_tac[`p === q`,`p'`] >>
   fs[entails_def,EQUATION_HAS_TYPE_BOOL] >>
-  imp_res_tac context_ok_sig >>
+  imp_res_tac theory_ok_sig >>
   fs[term_ok_equation] >>
   conj_asm1_tac >- metis_tac[ACONV_TYPE,WELLTYPED,WELLTYPED_LEMMA] >> rw[] >>
-  `term_ok (sigof ctxt) (p === q)` by metis_tac[term_ok_equation] >>
+  `term_ok (sigof thy) (p === q)` by metis_tac[term_ok_equation] >>
   imp_res_tac (UNDISCH termsem_equation) >> rfs[boolean_eq_true] >>
   metis_tac[termsem_aconv])
 
 val INST_correct = store_thm("INST_correct",
   ``is_set_theory ^mem ⇒
-    ∀ctxt h c.
+    ∀thy h c.
       (∀s s'. MEM (s',s) ilist ⇒
-              ∃x ty. (s = Var x ty) ∧ s' has_type ty ∧ term_ok (sigof ctxt) s') ∧
-      (ctxt, h) |= c
-    ⇒ (ctxt, MAP (VSUBST ilist) h) |= VSUBST ilist c``,
+              ∃x ty. (s = Var x ty) ∧ s' has_type ty ∧ term_ok (sigof thy) s') ∧
+      (thy, h) |= c
+    ⇒ (thy, MAP (VSUBST ilist) h) |= VSUBST ilist c``,
   rw[entails_def,EVERY_MAP,EVERY_MEM,satisfies_def] >>
   TRY ( match_mp_tac term_ok_VSUBST >> metis_tac[] ) >>
   TRY ( match_mp_tac VSUBST_HAS_TYPE >> metis_tac[] ) >>
   qspecl_then[`c`,`ilist`]mp_tac termsem_VSUBST >>
   discharge_hyps >- metis_tac[welltyped_def] >>
-  disch_then(qspecl_then[`sigof ctxt`,`i`,`v`]SUBST1_TAC) >>
+  disch_then(qspecl_then[`sigof thy`,`i`,`v`]SUBST1_TAC) >>
   first_x_assum(qspec_then`i`mp_tac) >> rw[] >>
   first_x_assum(match_mp_tac o MP_CANON) >>
   conj_tac >- (
-    Cases_on`v`>>
     fs[is_valuation_def] >>
     fs[is_term_valuation_def,APPLY_UPDATE_LIST_ALOOKUP,rich_listTheory.MAP_REVERSE] >>
     rw[] >>
@@ -199,32 +192,31 @@ val INST_correct = store_thm("INST_correct",
     rpt BasicProvers.VAR_EQ_TAC >>
     match_mp_tac (UNDISCH termsem_typesem) >>
     rw[is_valuation_def,is_term_valuation_def] >>
-    fs[is_model_def] >> metis_tac[is_std_interpretation_is_type] ) >>
+    fs[models_def] >> metis_tac[is_std_interpretation_is_type] ) >>
   fs[EVERY_MAP,EVERY_MEM] >>
   metis_tac[termsem_VSUBST,welltyped_def])
 
 val INST_TYPE_correct = store_thm("INST_TYPE_correct",
   ``is_set_theory ^mem ⇒
-    ∀ctxt h c.
-      EVERY (type_ok (types ctxt)) (MAP FST tyin) ∧
-      (ctxt, h) |= c
-    ⇒ (ctxt, MAP (INST tyin) h) |= INST tyin c``,
+    ∀thy h c.
+      EVERY (type_ok (tysof thy)) (MAP FST tyin) ∧
+      (thy, h) |= c
+    ⇒ (thy, MAP (INST tyin) h) |= INST tyin c``,
   rw[entails_def,EVERY_MAP,EVERY_MEM,satisfies_def] >>
   TRY ( match_mp_tac term_ok_INST >> fs[EVERY_MAP,EVERY_MEM] >> metis_tac[] ) >>
   TRY ( match_mp_tac INST_HAS_TYPE >> metis_tac[TYPE_SUBST_Bool] ) >>
-  qspecl_then[`sigof ctxt`,`c`,`tyin`]mp_tac termsem_INST >>
+  qspecl_then[`sigof thy`,`c`,`tyin`]mp_tac termsem_INST >>
   discharge_hyps >- metis_tac[welltyped_def] >>
   disch_then(qspecl_then[`i`,`v`]SUBST1_TAC) >>
   first_x_assum(qspec_then`i`mp_tac)>>rw[]>>
   first_x_assum(match_mp_tac o MP_CANON) >>
   conj_tac >- (
-    Cases_on`v`>>
     fs[is_valuation_def] >>
     conj_tac >- (
       fs[is_type_valuation_def] >> rw[] >>
       match_mp_tac (UNDISCH typesem_inhabited) >>
-      Cases_on`i`>>fs[is_model_def,is_interpretation_def] >>
-      qexists_tac`types ctxt` >> simp[is_type_valuation_def] >>
+      Cases_on`i`>>fs[models_def,is_interpretation_def] >>
+      qexists_tac`tysof thy` >> simp[is_type_valuation_def] >>
       fs[FORALL_PROD] >>
       metis_tac[holSyntaxLibTheory.REV_ASSOCD_MEM,type_ok_def] ) >>
     fs[is_term_valuation_def,APPLY_UPDATE_LIST_ALOOKUP,rich_listTheory.MAP_REVERSE] >>
@@ -235,15 +227,15 @@ val INST_TYPE_correct = store_thm("INST_TYPE_correct",
 
 val MK_COMB_correct = store_thm("MK_COMB_correct",
   ``is_set_theory ^mem ⇒
-    ∀ctxt h1 h2 l1 r1 l2 r2.
-      (ctxt,h1) |= l1 === r1 ∧ (ctxt,h2) |= l2 === r2 ∧
+    ∀thy h1 h2 l1 r1 l2 r2.
+      (thy,h1) |= l1 === r1 ∧ (thy,h2) |= l2 === r2 ∧
       welltyped (Comb l1 l2)
-      ⇒ (ctxt,TERM_UNION h1 h2) |= Comb l1 l2 === Comb r1 r2``,
+      ⇒ (thy,TERM_UNION h1 h2) |= Comb l1 l2 === Comb r1 r2``,
   rw[] >>
   match_mp_tac (UNDISCH binary_inference_rule) >>
   map_every qexists_tac[`l1 === r1`,`l2 === r2`] >>
   fs[entails_def] >>
-  imp_res_tac context_ok_sig >>
+  imp_res_tac theory_ok_sig >>
   conj_asm1_tac >- (
     fs[EQUATION_HAS_TYPE_BOOL,term_ok_equation] >>
     metis_tac[] ) >>
@@ -256,30 +248,30 @@ val MK_COMB_correct = store_thm("MK_COMB_correct",
 
 val REFL_correct = store_thm("REFL_correct",
   ``is_set_theory ^mem ⇒
-    ∀ctxt t.
-      context_ok ctxt ∧ term_ok (sigof ctxt) t ⇒
-      (ctxt,[]) |= t === t``,
+    ∀thy t.
+      theory_ok thy ∧ term_ok (sigof thy) t ⇒
+      (thy,[]) |= t === t``,
   rw[] >>
   simp[entails_def,EQUATION_HAS_TYPE_BOOL] >>
-  imp_res_tac context_ok_sig >>
+  imp_res_tac theory_ok_sig >>
   imp_res_tac term_ok_welltyped >>
   conj_asm1_tac >- rw[term_ok_equation] >>
   rw[satisfies_def] >>
-  `is_structure (sigof ctxt) i v` by (
-    rw[is_structure_def] >> fs[is_model_def] ) >>
+  `is_structure (sigof thy) i v` by (
+    rw[is_structure_def] >> fs[models_def] ) >>
   imp_res_tac termsem_equation >>
   rw[boolean_def])
 
 val TRANS_correct = store_thm("TRANS_correct",
   ``is_set_theory ^mem ⇒
-    ∀ctxt h1 h2 l m1 m2 r.
-      (ctxt,h1) |= l === m1 ∧ (ctxt,h2) |= m2 === r ∧ ACONV m1 m2
-      ⇒ (ctxt,TERM_UNION h1 h2) |= l === r``,
+    ∀thy h1 h2 l m1 m2 r.
+      (thy,h1) |= l === m1 ∧ (thy,h2) |= m2 === r ∧ ACONV m1 m2
+      ⇒ (thy,TERM_UNION h1 h2) |= l === r``,
   strip_tac >>
   rw[] >> match_mp_tac (UNDISCH binary_inference_rule) >>
   map_every qexists_tac[`l === m1`,`m2 === r`] >>
   fs[entails_def] >>
-  imp_res_tac context_ok_sig >>
+  imp_res_tac theory_ok_sig >>
   conj_asm1_tac >- (
     fs[EQUATION_HAS_TYPE_BOOL] >>
     metis_tac[ACONV_TYPE] ) >>
@@ -290,6 +282,22 @@ val TRANS_correct = store_thm("TRANS_correct",
   rfs[boolean_eq_true] >> fs[term_ok_equation] >>
   metis_tac[termsem_aconv,ACONV_SYM,term_ok_welltyped])
 
+val proves_sound = store_thm("proves_sound",
+  ``is_set_theory ^mem ⇒ ∀thyh c. thyh |- c ⇒ thyh |= c``,
+  strip_tac >> match_mp_tac proves_ind >>
+  conj_tac >- metis_tac[ABS_correct] >>
+  conj_tac >- metis_tac[ASSUME_correct] >>
+  conj_tac >- metis_tac[BETA_correct] >>
+  conj_tac >- metis_tac[DEDUCT_ANTISYM_correct] >>
+  conj_tac >- metis_tac[EQ_MP_correct] >>
+  conj_tac >- metis_tac[INST_correct] >>
+  conj_tac >- metis_tac[INST_TYPE_correct] >>
+  conj_tac >- metis_tac[MK_COMB_correct] >>
+  conj_tac >- metis_tac[REFL_correct] >>
+  conj_tac >- metis_tac[TRANS_correct] >>
+  rw[entails_def,theory_ok_def,models_def])
+
+(*
 val new_axiom_correct = store_thm("new_axiom_correct",
   ``∀ctxt p h c.
     p has_type Bool ∧ term_ok (sigof ctxt) p ∧
@@ -501,24 +509,6 @@ val new_type_definition_correct = store_thm("new_type_definition_correct",
   fs[entails_def] >- (
       metis_tac[satisfies_extend,SUBMAP_REFL,EVERY_DEF] ) >>
   fs[is_model_def,EVERY_MEM])
-
-val soundness = store_thm("soundness",
-  ``is_set_theory ^mem ⇒ ∀ctxtasl p. ctxtasl |- p ⇒ ctxtasl |= p``,
-  strip_tac >> match_mp_tac proves_ind >>
-  conj_tac >- metis_tac[ABS_correct] >>
-  conj_tac >- metis_tac[ASSUME_correct] >>
-  conj_tac >- metis_tac[BETA_correct] >>
-  conj_tac >- metis_tac[DEDUCT_ANTISYM_correct] >>
-  conj_tac >- metis_tac[EQ_MP_correct] >>
-  conj_tac >- metis_tac[INST_correct] >>
-  conj_tac >- metis_tac[INST_TYPE_correct] >>
-  conj_tac >- metis_tac[MK_COMB_correct] >>
-  conj_tac >- metis_tac[REFL_correct] >>
-  conj_tac >- metis_tac[TRANS_correct] >>
-  conj_tac >- metis_tac[new_axiom_correct] >>
-  conj_tac >- metis_tac[new_constant_correct] >>
-  conj_tac >- metis_tac[new_specification_correct] >>
-  conj_tac >- metis_tac[new_type_correct] >>
-  metis_tac[new_type_definition_correct])
+*)
 
 val _ = export_theory()
